Proving LRbind

TypeSoundness.v
@@ -260,8 +260,8 @@ Infix "≤" := le (at level 70).
 
 Infix "×" := Tprod (at level 40) : ty.
 Infix "+" := Tsum : ty.
-Definition runsto e τ := IsValue e /\ |- e τ.
-Infix "↓" := runsto (at level 51).
+Definition valueOf e τ := IsValue e /\ |- e τ.
+Infix "↓" := valueOf (at level 51).
 
 Local Open Scope prog_scope.
 
@@ -436,7 +436,13 @@ Notation "▹" := Rlater : rel.
 Delimit Scope rel with rel.
 Bind Scope rel with rel.
 
-Definition typingew (ew : wexpr) τ := let (e, w) := ew in e ↓ τ /\ wtyping [] w !τ.
+Definition IsWValue : forall t ctx, open_width t ctx -> Prop.
+  admit.
+Qed.
+
+Definition wrunsto {t} (w w' : open_width t []) := (wsteps w w' /\ IsWValue w')%type.
+Definition wvalueOf (w : width) τ := wtyping [] w !τ /\ IsWValue w.
+Definition typingew (ew : wexpr) τ := let (e, w) := ew in e ↓ τ /\ wvalueOf w τ.
 Infix "↓↓" := typingew (at level 51).
 
 Module test_rel.
@@ -674,8 +680,8 @@ Section LR.
     \ew, let (e, w) := ew in
          ⌈|- e (ρ $ τ) /\ wtyping [] w !(ρ $ τ) /\
          exists B, wsteps wB (Wconst B) /\ forall n e', (~>## e n 0 e') -> n ≤ B⌉%type /\ 
-         ⌈exists v, e ⇓ v⌉ /\
-         (∀v, ⌈e ⇓ v⌉ ===> (v, w) ∈ relV ctx ρ /\ ⌈!v ≤ s⌉) /\
+         ⌈exists v w', e ⇓ v /\ wrunsto w w'⌉%type /\
+         (∀v w', ⌈e ⇓ v /\ wrunsto w w'⌉%type ===> (v, w') ∈ relV ctx ρ /\ ⌈!v ≤ s⌉) /\
          (∀e', ⌈~>*# e 1 e'⌉ ===> 
                      match c with
                        | 0 => ⊥
@@ -1331,8 +1337,8 @@ Lemma openup8_imply ctx t1 t2 t3 t4 t5 t6 t7 t8 (f g : t1 -> t2 -> t3 -> t4 -> t
   admit.
 Qed.
 
-Lemma openup4_forall1_elim t1 t2 t3 t4 ctx (f : t1 -> t2 -> t3 -> t4 -> wexpr -> rel 0 ctx) ctxfo x1 x2 x3 x4 e w Ps Q :
-  openup6 (ctx := ctxfo) (fun x1 x2 x3 x4 w e => f x1 x2 x3 x4 (e, w)) x1 x2 x3 x4 w e :: Ps |~ Q ->
+Lemma openup4_forall1_elim t1 t2 t3 t4 t ctx (f : t1 -> t2 -> t3 -> t4 -> t -> rel 0 ctx) ctxfo x1 x2 x3 x4 x Ps Q :
+  openup5 (ctx := ctxfo) f x1 x2 x3 x4 x :: Ps |~ Q ->
   openup4 (fun x1 x2 x3 x4 => ∀x, f x1 x2 x3 x4 x) x1 x2 x3 x4 :: Ps |~ Q.
   admit.
 Qed.
@@ -1790,10 +1796,20 @@ Proof.
     [] |~~ 
        ⌈|- e (ρ $ τ) /\ wtyping [] w !(ρ $ τ) ⌉ /\
        ⌈exists B, wsteps wB (Wconst B) /\ forall n e', (~>## e n 0 e') -> n ≤ B⌉%type /\ 
-       ⌈exists v, e ⇓ v⌉ /\
-       (∀v, ⌈e ⇓ v⌉ ===> (v, w) ∈ relV τ ρ /\ ⌈!v ≤ s⌉) /\
+       ⌈exists v w', e ⇓ v /\ wrunsto w w'⌉%type /\
+       (∀v w', ⌈e ⇓ v /\ wrunsto w w'⌉%type ===> (v, w') ∈ relV τ ρ /\ ⌈!v ≤ s⌉) /\
        (∀e', ⌈~>*# e 1 e'⌉ ===> ⌈0 < c⌉ /\ ▹ [] ((e', w) ∈ relE τ wB (c - 1) s ρ)) ===>
        (e, w) ∈ relE τ wB c s ρ.
+    admit.
+  Qed.
+  Lemma relE_elim lctx ctx e w τ wB c s (ρ : csubsts lctx ctx) :
+    [] |~~ 
+       (e, w) ∈ relE τ wB c s ρ ===>
+       ⌈|- e (ρ $ τ) /\ wtyping [] w !(ρ $ τ) ⌉ /\
+       ⌈exists B, wsteps wB (Wconst B) /\ forall n e', (~>## e n 0 e') -> n ≤ B⌉%type /\ 
+       ⌈exists v w', e ⇓ v /\ wrunsto w w'⌉%type /\
+       (∀v w', ⌈e ⇓ v /\ wrunsto w w'⌉%type ===> (v, w') ∈ relV τ ρ /\ ⌈!v ≤ s⌉) /\
+       (∀e', ⌈~>*# e 1 e'⌉ ===> ⌈0 < c⌉ /\ ▹ [] ((e', w) ∈ relE τ wB (c - 1) s ρ)).
     admit.
   Qed.
   Lemma openup3_apply ctx t1 t2 t3 (f g : t1 -> t2 -> t3 -> rel 0 ctx) ctxfo x1 x2 x3 Ps : 
@@ -1815,7 +1831,258 @@ Proof.
   rewrite openup3_and.
   eapply rsplit.
   {
-    admit. 
+    subst Ps.
+    Lemma openup4_apply ctx t1 t2 t3 t4 (f g : t1 -> t2 -> t3 -> t4 -> rel 0 ctx) ctxfo x1 x2 x3 x4 Ps : 
+      (forall x1 x2 x3 x4, [] |~~ f x1 x2 x3 x4 ===> g x1 x2 x3 x4) ->
+      Ps |~ openup4 (ctx := ctxfo) f x1 x2 x3 x4 ->
+      Ps |~ openup4 (ctx := ctxfo) g x1 x2 x3 x4.
+      admit.
+    Qed.
+    Lemma openup4_apply_in ctx t1 t2 t3 t4 (f g : t1 -> t2 -> t3 -> t4 -> rel 0 ctx) ctxfo x1 x2 x3 x4 Ps P : 
+      (forall x1 x2 x3 x4, [] |~~ f x1 x2 x3 x4 ===> g x1 x2 x3 x4) ->
+      openup4 (ctx := ctxfo) g x1 x2 x3 x4 :: Ps |~ P ->
+      openup4 (ctx := ctxfo) f x1 x2 x3 x4 :: Ps |~ P.
+      admit.
+    Qed.
+    eapply openup4_apply_in.
+    {
+      intros.
+      eapply relE_elim.
+    }
+    rewrite openup4_and.
+    eapply destruct_and.
+    eapply totop with (n := 1); [ reflexivity | unfold removen ].
+    rewrite openup4_and.
+    eapply destruct_and.
+    eapply totop with (n := 1); [ reflexivity | unfold removen ].
+    rewrite openup4_and.
+    eapply destruct_and.
+    eapply totop with (n := 1); [ reflexivity | unfold removen ].
+    rewrite openup4_and.
+    eapply destruct_and.
+    eapply totop with (n := 2); [ reflexivity | unfold removen ].
+    rewrite openup4_totop2.
+    rewrite openup4_openup3.
+    Lemma openup3_totop1 {t0 t1 t2 t3} {f : t0 -> t1 -> t2 -> t3} {ctxfo x0 x1 x2} : openup3 (ctx := ctxfo) f x0 x1 x2 = openup3 (fun x1 x0 x2 => f x0 x1 x2) x1 x0 x2.
+      admit.
+    Qed.
+    Lemma openup3_totop2 {t0 t1 t2 t3} {f : t0 -> t1 -> t2 -> t3} {ctxfo x0 x1 x2} : openup3 (ctx := ctxfo) f x0 x1 x2 = openup3 (fun x2 x0 x1 => f x0 x1 x2) x2 x0 x1.
+      admit.
+    Qed.
+    Lemma openup3_openup2 t1 t2 t3 t4 (f : t2 -> t3 -> t4) ctxfo x1 x2 x3 : openup3 (ctx := ctxfo) (fun (_ : t1) x2 x3 => f x2 x3) x1 x2 x3 = openup2 f x2 x3.
+      admit.
+    Qed.
+    rewrite openup3_totop2.
+    rewrite openup3_openup2.
+    Lemma openup2_totop1 {t0 t1 t2} {f : t0 -> t1 -> t2} {ctxfo x0 x1} : openup2 (ctx := ctxfo) f x0 x1 = openup2 (fun x1 x0 => f x0 x1) x1 x0.
+      admit.
+    Qed.
+    Lemma openup2_openup1 t1 t2 t3 (f : t2 -> t3) ctxfo x1 x2 : openup2 (ctx := ctxfo) (fun (_ : t1) x2 => f x2) x1 x2 = openup1 f x2.
+      admit.
+    Qed.
+    Notation "[| P |]" := (Rinj P) (only parsing) : rel.
+    Lemma inj_exists_elim T (P : T -> Prop) ctx :
+      [] |~~ [| exists x, P x |] ===> ∃x, [| P x |] : rel 0 ctx.
+      admit.
+    Qed.
+    Lemma openup1_apply_in ctx t1 (f g : t1 -> rel 0 ctx) ctxfo x1 Ps P : 
+      (forall x1, [] |~~ f x1 ===> g x1) ->
+      openup1 (ctx := ctxfo) g x1 :: Ps |~ P ->
+      openup1 (ctx := ctxfo) f x1 :: Ps |~ P.
+      admit.
+    Qed.
+    Lemma openup2_apply_in ctx t1 t2 (f g : t1 -> t2 -> rel 0 ctx) ctxfo x1 x2 Ps P : 
+      (forall x1 x2, [] |~~ f x1 x2 ===> g x1 x2) ->
+      openup2 (ctx := ctxfo) g x1 x2 :: Ps |~ P ->
+      openup2 (ctx := ctxfo) f x1 x2 :: Ps |~ P.
+      admit.
+    Qed.
+    eapply openup2_apply_in.
+    {
+      intros.
+      eapply inj_exists_elim.
+    }
+    Lemma openup1_exists1_elim ctxfo ctx t1 t (Q : open_rel ctxfo 0 ctx) (f : t1 -> t -> rel 0 ctx) x1 (Ps : list (open_rel ctxfo 0 ctx)) :
+      openup2 (fun x1 x => f x1 x) (lift (new := [_]) x1) V0 :: liftPs (new := [_]) Ps |~ lift Q ->
+      openup1 (fun x1 => ∃x, f x1 x) x1 :: Ps |~ Q.
+      admit.
+    Qed.
+    Lemma openup2_exists1_elim ctxfo ctx t1 t2 t (Q : open_rel ctxfo 0 ctx) (f : t1 -> t2 -> t -> rel 0 ctx) x1 x2 (Ps : list (open_rel ctxfo 0 ctx)) :
+      openup3 (fun x1 x2 x => f x1 x2 x) (lift (new := [_]) x1) (lift x2) V0 :: liftPs (new := [_]) Ps |~ lift Q ->
+      openup2 (fun x1 x2 => ∃x, f x1 x2 x) x1 x2 :: Ps |~ Q.
+      admit.
+    Qed.
+    eapply openup2_exists1_elim.
+    Lemma openup3_apply_in ctx t1 t2 t3 (f g : t1 -> t2 -> t3 -> rel 0 ctx) ctxfo x1 x2 x3 Ps P : 
+      (forall x1 x2 x3, [] |~~ f x1 x2 x3 ===> g x1 x2 x3) ->
+      openup3 (ctx := ctxfo) g x1 x2 x3 :: Ps |~ P ->
+      openup3 (ctx := ctxfo) f x1 x2 x3 :: Ps |~ P.
+      admit.
+    Qed.
+    eapply openup3_apply_in.
+    {
+      intros.
+      eapply inj_exists_elim.
+    }
+    eapply openup3_exists1_elim.
+    repeat rewrite liftPs_cons.
+    repeat rewrite lift_openup4.
+    combine_lift.
+    rewrite lift_openup3.
+    unfold liftPs, liftPs1, map.
+    Lemma dup_premise ctxfo ctx (P Q : open_rel ctxfo 0 ctx) Ps :
+      P :: P :: Ps |~ Q ->
+      P :: Ps |~ Q.
+      admit.
+    Qed.
+    eapply dup_premise.
+    eapply totop with (n := 2); [ reflexivity | unfold removen ].
+    rewrite openup4_totop2.
+    rewrite openup4_openup3.
+    rewrite openup3_totop2.
+    rewrite openup3_openup2.
+    Lemma openup2_forall1_elim t1 t2 t ctx (f : t1 -> t2 -> t -> rel 0 ctx) ctxfo x1 x2 x Ps Q :
+      openup3 (ctx := ctxfo) f x1 x2 x :: Ps |~ Q ->
+      openup2 (fun x1 x2 => ∀x, f x1 x2 x) x1 x2 :: Ps |~ Q.
+      admit.
+    Qed.
+    Lemma openup3_forall1_elim t1 t2 t3 t ctx (f : t1 -> t2 -> t3 -> t -> rel 0 ctx) ctxfo x1 x2 x3 x Ps Q :
+      openup4 (ctx := ctxfo) f x1 x2 x3 x :: Ps |~ Q ->
+      openup3 (fun x1 x2 x3 => ∀x, f x1 x2 x3 x) x1 x2 x3 :: Ps |~ Q.
+      admit.
+    Qed.
+    eapply openup2_forall1_elim with (x := V1).
+    eapply openup3_forall1_elim with (x := V0).
+    Lemma openup3_imply {ctx t1 t2 t3} {f g : t1 -> t2 -> t3 -> rel 0 ctx} {ctxfo x1 x2 x3} : openup3 (ctx := ctxfo) (fun x1 x2 x3 => f x1 x2 x3 ===> g x1 x2 x3) x1 x2 x3 == (openup3 f x1 x2 x3 ===> openup3 g x1 x2 x3)%OR.
+      (* should be eq *)
+      admit.
+    Qed.
+    Lemma eqv_premise ctxfo ctx (P P' Q : open_rel ctxfo 0 ctx) Ps :
+      P == P' ->
+      P' :: Ps |~ Q ->
+      P :: Ps |~ Q.
+      admit.
+    Qed.
+    eapply eqv_premise.
+    {
+      eapply openup4_imply.
+    }
+    eapply imply_elim.
+    rewrite openup4_openup3.
+    rewrite openup3_openup2.
+    Lemma openup2_and ctx t1 t2 (f g : t1 -> t2 -> rel 0 ctx) ctxfo x1 x2 : openup2 (ctx := ctxfo) (fun x1 x2 => f x1 x2 /\ g x1 x2) x1 x2 == (openup2 f x1 x2 /\ openup2 g x1 x2)%OR.
+      admit.
+    Qed.
+    rewrite openup2_and.
+    eapply destruct_and.
+    eapply totop with (n := 6); [ reflexivity | unfold removen ].
+    Lemma openup5_forall1_elim t1 t2 t3 t4 t5 t ctx (f : t1 -> t2 -> t3 -> t4 -> t5 -> t -> rel 0 ctx) ctxfo x1 x2 x3 x4 x5 x Ps Q :
+      openup6 (ctx := ctxfo) f x1 x2 x3 x4 x5 x :: Ps |~ Q ->
+      openup5 (fun x1 x2 x3 x4 x5 => ∀x, f x1 x2 x3 x4 x5 x) x1 x2 x3 x4 x5 :: Ps |~ Q.
+      admit.
+    Qed.
+    rewrite openup4_totop2.
+    rewrite openup4_openup3.
+    rewrite openup3_totop2.
+    rewrite openup3_openup2.
+    eapply dup_premise.
+    unfold relEC.
+    eapply openup2_forall1_elim with (x := V1).
+    eapply openup3_forall1_elim with (x := V0).
+    eapply eqv_premise.
+    {
+      eapply openup4_imply.
+    }
+    Lemma imply_eelim ctxfo ctx (P Q : open_rel ctxfo 0 ctx) Ps G : 
+      Ps |~ P ->
+      Q :: Ps |~ G ->
+      (P ===> Q)%OR :: Ps |~ G.
+      admit.
+    Qed.
+    eapply imply_eelim.
+    {
+      rewrite openup4_and.
+      eapply rsplit.
+      {
+        repeat rewrite openup4_openup3.
+        repeat rewrite openup3_openup2.
+        eapply totop with (n := 1); [ reflexivity | unfold removen ].
+        eapply ctx_refl.
+      }
+      admit. (* ⌈x1 ~>* x3 /\ !x3 ≤ s₁ /\ wsteps x2 x4⌉ *)
+    }
+    rewrite openup4_openup3.
+    rewrite openup3_openup2.
+    rewrite openup2_totop1.
+    rewrite openup2_openup1.
+    eapply openup1_apply_in.
+    {
+      intros.
+      eapply relE_elim.
+    }
+    Lemma openup1_and ctx t1 (f g : t1 -> rel 0 ctx) ctxfo x1 : openup1 (ctx := ctxfo) (fun x1 => f x1 /\ g x1) x1 == (openup1 f x1 /\ openup1 g x1)%OR.
+      admit.
+    Qed.
+    eapply eqv_premise; [ eapply openup1_and | ].
+    eapply destruct_and.
+    eapply totop with (n := 1); [ reflexivity | unfold removen ].
+    eapply eqv_premise; [ eapply openup1_and | ].
+    eapply destruct_and.
+    eapply openup1_apply_in.
+    {
+      intros.
+      eapply inj_exists_elim.
+    }
+    eapply openup1_exists1_elim.
+    repeat rewrite liftPs_cons.
+    repeat rewrite lift_openup4.
+    combine_lift.
+    unfold liftPs, liftPs1, map.
+    eapply totop with (n := 8); [ reflexivity | unfold removen ].
+    rewrite openup4_totop1.
+    rewrite openup4_openup3.
+    rewrite openup3_totop1.
+    rewrite openup3_openup2.
+    eapply openup2_apply_in.
+    {
+      intros.
+      eapply inj_exists_elim.
+    }
+    eapply openup2_exists1_elim.
+    repeat rewrite liftPs_cons.
+    repeat rewrite lift_openup4.
+    combine_lift.
+    unfold liftPs, liftPs1, map.
+    repeat erewrite lift_openup3.
+    set (Ps := [_;_;_;_;_;_;_;_;_;_;_;_]).
+    rewrite openup3_totop1.
+    rewrite openup3_openup2.
+    Lemma inj_exists_intro T (P : T -> Prop) ctx :
+      [] |~~ (∃x, [| P x |] : rel 0 ctx) ===> [| exists x, P x |].
+      admit.
+    Qed.
+    Lemma openup2_apply ctx t1 t2 (f g : t1 -> t2 -> rel 0 ctx) ctxfo x1 x2 Ps : 
+      (forall x1 x2, [] |~~ f x1 x2 ===> g x1 x2) ->
+      Ps |~ openup2 (ctx := ctxfo) f x1 x2 ->
+      Ps |~ openup2 (ctx := ctxfo) g x1 x2.
+      admit.
+    Qed.
+    eapply openup2_apply.
+    {
+      intros.
+      eapply inj_exists_intro.
+    }
+    Lemma openup2_exists1 ctx t t1 t2 (f : t -> t1 -> t2 -> rel 0 ctx) ctxfo x x1 x2 Ps : 
+      Ps |~ openup3 f x x1 x2 ->
+      Ps |~ openup2 (ctx := ctxfo) (fun x1 x2 => ∃x, f x x1 x2) x1 x2.
+      admit.
+    Qed.
+    eapply openup2_exists1 with (x := openup2 add V0 V1).
+    Lemma openup3_comp_openup2 t1 t2 t3 t4 (f : t1 -> t2 -> t3 -> t4) A1 A2 (g : A1 -> A2 -> t1) ctxfo x2 x3 y1 y2 : openup3 (ctx := ctxfo) (fun x1 x2 x3 => f x1 x2 x3) (openup2 (fun y1 y2 => g y1 y2) y1 y2) x2 x3 = openup4 (fun y1 y2 x2 x3 => f (g y1 y2) x2 x3) y1 y2 x2 x3.
+      admit.
+    Qed.
+    erewrite openup3_comp_openup2.
+    (*here*)
   }
   rewrite openup3_and.
   eapply rsplit.
@@ -2147,7 +2414,20 @@ Proof.
         rewrite openup5_openup4.
         rewrite openup4_totop1.
 
-        eapply openup4_forall1_elim with (e := V4) (w := V3).
+        Lemma openup4_forall1_elim' t1 t2 t3 t4 ctx (f : t1 -> t2 -> t3 -> t4 -> wexpr -> rel 0 ctx) ctxfo x1 x2 x3 x4 e w Ps Q :
+          openup6 (ctx := ctxfo) (fun x1 x2 x3 x4 w e => f x1 x2 x3 x4 (e, w)) x1 x2 x3 x4 w e :: Ps |~ Q ->
+          openup4 (fun x1 x2 x3 x4 => ∀x, f x1 x2 x3 x4 x) x1 x2 x3 x4 :: Ps |~ Q.
+        Proof.
+          intros H.
+          eapply openup4_forall1_elim with (x := openup2 pair e w).
+          rewrite openup5_totop4.
+          rewrite openup5_comp_openup2.
+          rewrite openup6_totop1.
+          do 4 rewrite openup6_totop5.
+          eauto.
+        Qed.
+
+        eapply openup4_forall1_elim' with (e := V4) (w := V3).
         rewrite openup6_imply.
         rewrite openup6_openup5.
         rewrite openup5_totop1.
